formalization/OperationalSemantics.v
@@ -1,66 +1,67 @@
 From stdpp Require Import mapset.
 From CT Require Import CoreLang.
 From CT Require Import CoreLangProp.
-From CT Require Import Trace.
 
 Import Atom.
 Import CoreLang.
 Import Tactics.
 Import NamelessTactics.
 
+Inductive eval_op: effop -> constant -> constant -> Prop :=
+| eval_op_plus_one: forall (a: nat), eval_op op_plus_one a (1 + a)
+| eval_op_eq_zero: forall (a: nat), eval_op op_eq_zero a (Nat.eqb a 0)
+| eval_op_rannat: forall (a b: nat), eval_op op_rannat a b.
+
+Global Hint Constructors eval_op: core.
+
+Notation "'⇓{' op '~' c1 '}{' c '}' " := (eval_op op c1 c)
+                                           (at level 30, format "⇓{ op ~ c1 }{ c }", c1 constr, c constr).
+
 (** This file defines the operational semantics of the core language. *)
 
-Reserved Notation "α '⊧' t1 '↪{' β '}' t2" (at level 60, t1 constr, β constr).
+Reserved Notation "t1 '↪' t2" (at level 60, t1 constr, t2 constr).
 
-(** the small step operational semantics (Fig. 3) *)
-(* Because in this formalization, we treat pure operations as effectful
-operations, the rule [STPureOp] is not necessary. *)
-Inductive step : list evop -> tm -> list evop -> tm -> Prop :=
-| STEffOp: forall (α β: list evop) op (c1 c: constant) e,
+Inductive step : tm -> tm -> Prop :=
+| STEffOp: forall op (c1 c: constant) e,
     body e -> lc c1 -> lc c ->
-    α ⊧{ op ~ c1 }⇓{ β }{ c } ->
-    α ⊧ (tleteffop op c1 e) ↪{ β } (e ^t^ c)
-| STLetE1: forall α β e1 e1' e,
+    ⇓{op ~ c1}{c} -> (tleteffop op c1 e) ↪ (e ^t^ c)
+| STLetE1: forall e1 e1' e,
     body e ->
-    α ⊧ e1 ↪{β} e1' ->
-    α ⊧ (tlete e1 e) ↪{β} (tlete e1' e)
-| STLetE2: forall α (v1: value) e,
+    e1 ↪ e1' ->
+    (tlete e1 e) ↪ (tlete e1' e)
+| STLetE2: forall (v1: value) e,
     lc v1 -> body e ->
-    α ⊧ (tlete (treturn v1) e) ↪{ α } (e ^t^ v1)
-| STLetAppLam: forall α T (v_x: value) e1 e,
+    (tlete (treturn v1) e) ↪ (e ^t^ v1)
+| STLetAppLam: forall T (v_x: value) e1 e,
     body e1 -> body e -> lc v_x ->
-    α ⊧ (tletapp (vlam T e1) v_x e) ↪{ α } tlete (e1 ^t^ v_x) e
-| STLetAppFix: forall α T_f (v_x: value) (e1: tm) e,
+    (tletapp (vlam T e1) v_x e) ↪ tlete (e1 ^t^ v_x) e
+| STLetAppFix: forall T_f (v_x: value) (e1: tm) e,
     body (vlam T_f e1) -> lc v_x -> body e ->
-    α ⊧ tletapp (vfix T_f (vlam T_f e1)) v_x e ↪{ α }
-            tletapp ((vlam T_f e1) ^v^ v_x) (vfix T_f (vlam T_f e1)) e
-| STMatchbTrue: forall α e1 e2,
+    tletapp (vfix T_f (vlam T_f e1)) v_x e ↪
+      tletapp ((vlam T_f e1) ^v^ v_x) (vfix T_f (vlam T_f e1)) e
+| STMatchbTrue: forall e1 e2,
     lc e1 -> lc e2 ->
-    α ⊧ (tmatchb true e1 e2) ↪{ α } e1
-| STMatchbFalse: forall α e1 e2,
+    (tmatchb true e1 e2) ↪ e1
+| STMatchbFalse: forall e1 e2,
     lc e1 -> lc e2 ->
-    α ⊧ (tmatchb false e1 e2) ↪{ α } e2
-where "α '⊧' t1 '↪{' β '}' t2" := (step α t1 β t2).
+    (tmatchb false e1 e2) ↪ e2
+where "t1 '↪' t2" := (step t1 t2).
 
-Inductive multistep : list evop -> tm -> list evop -> tm -> Prop :=
-| multistep_refl : forall α (e : tm),
-    lc e -> multistep α e α e
-| multistep_step : forall  α β γ (x y z: tm),
-    α ⊧ x ↪{ β } y ->
-    multistep β y γ z ->
-    multistep α x γ z.
+Inductive multistep : tm -> tm -> Prop :=
+| multistep_refl : forall (e : tm),
+    lc e -> multistep e e
+| multistep_step : forall (x y z: tm),
+    x ↪ y ->
+    multistep y z ->
+    multistep x z.
 
-Notation "α '⊧' t1 '↪*{' β '}' t2" := (multistep α t1 β t2) (at level 60, t1 constr, β constr).
-
-Definition pure_multistep (t1 t2: tm) := forall α, α ⊧ t1 ↪*{ α } t2.
-
-Notation "t1 '↪*' t2" := (pure_multistep t1 t2) (at level 60, t1 constr, t2 constr).
+Notation " t1 '↪*' t2" := (multistep t1 t2) (at level 60, t1 constr, t2 constr).
 
 Global Hint Constructors multistep : core.
 
 (** * Properties of operational semantics *)
 
-Lemma step_regular: forall α β e1 e2, α ⊧ e1 ↪{ β } e2 -> lc e1 /\ lc e2.
+Lemma step_regular: forall e1 e2, e1 ↪ e2 -> lc e1 /\ lc e2.
 Proof.
   intros.
   induction H; split; auto.
@@ -78,12 +79,12 @@ Proof.
     + rewrite body_vlam_eq in H. rewrite lc_fix_iff_body; eauto.
 Qed.
 
-Lemma step_regular1: forall α β e1 e2, α ⊧ e1 ↪{ β } e2 -> lc e1.
+Lemma step_regular1: forall e1 e2, e1 ↪ e2 -> lc e1.
 Proof.
   intros. apply step_regular in H. destruct H; auto.
 Qed.
 
-Lemma step_regular2: forall α β e1 e2, α ⊧ e1 ↪{ β } e2 -> lc e2.
+Lemma step_regular2: forall e1 e2, e1 ↪ e2 -> lc e2.
 Proof.
   intros. apply step_regular in H. destruct H; auto.
 Qed.
@@ -91,60 +92,53 @@ Qed.
 Global Hint Resolve step_regular1: core.
 Global Hint Resolve step_regular2: core.
 
-Theorem multistep_trans :
-  forall α βx βy (x y z : tm),
-   α ⊧ x ↪*{ βx } y ->
-   βx ⊧ y ↪*{ βy } z ->
-   α ⊧ x ↪*{ βy } z.
+Theorem multistep_trans: forall (x y z : tm), x ↪* y -> y ↪* z -> x ↪* z.
 Proof.
   intros. generalize dependent z.
   induction H; intros; eauto.
 Qed.
 
-Theorem multistep_R : forall α β (x y : tm),
-    α ⊧ x ↪{ β } y -> α ⊧ x ↪*{ β } y.
+Theorem multistep_R : forall (x y : tm),
+    x ↪ y -> x ↪* y.
 Proof. intros. eauto.
 Qed.
 
-Lemma multi_step_regular: forall α β e1 e2, α ⊧ e1 ↪*{ β } e2 -> lc e1 /\ lc e2.
+Lemma multi_step_regular: forall e1 e2, e1 ↪* e2 -> lc e1 /\ lc e2.
 Proof.
   induction 1; intuition eauto.
 Qed.
 
-Lemma multi_step_regular1: forall α β e1 e2, α ⊧ e1 ↪*{ β } e2 -> lc e1.
+Lemma multi_step_regular1: forall e1 e2, e1 ↪* e2 -> lc e1.
 Proof.
   intros. apply multi_step_regular in H. destruct H; auto.
 Qed.
 
-Lemma multi_step_regular2: forall α β e1 e2, α ⊧ e1 ↪*{ β } e2 ->  lc e2.
+Lemma multi_step_regular2: forall e1 e2, e1 ↪* e2 ->  lc e2.
 Proof.
   intros. apply multi_step_regular in H. destruct H; auto.
 Qed.
 
 Ltac step_regular_simp :=
   repeat match goal with
-    | [H: _ ⊧ _ ↪*{ _ } _ |- lc _ ] => apply multi_step_regular in H; destruct H; auto
-    | [H: _ ⊧ _ ↪{ _ } _ |- lc _ ] => apply step_regular in H; destruct H; auto
-    | [H: _ ⊧ _ ↪*{ _ } _ |- body _] => apply multi_step_regular in H; destruct H; auto
-    | [H: _ ⊧ _ ↪{ _ } _ |- body _] => apply step_regular in H; destruct H; auto
+    | [H: _ ↪* _ |- lc _ ] => apply multi_step_regular in H; destruct H; auto
+    | [H: _ ↪ _ |- lc _ ] => apply step_regular in H; destruct H; auto
+    | [H: _ ↪* _ |- body _] => apply multi_step_regular in H; destruct H; auto
+    | [H: _ ↪ _ |- body _] => apply step_regular in H; destruct H; auto
     end.
 
-Lemma value_reduction_refl: forall α β (v1: value) v2, α ⊧ v1 ↪*{ β} v2 -> v2 = v1 /\ β = α.
+Lemma value_reduction_refl: forall (v1: value) v2, v1 ↪* v2 -> v2 = v1.
 Proof.
-  intros * H.
-  sinvert H; easy.
+  intros * H. sinvert H; easy.
 Qed.
 
 Ltac reduction_simp :=
   match goal with
-  | H: _ ⊧ (treturn _) ↪*{ _ } _  |- _ =>
+  | H: (treturn _) ↪* _  |- _ =>
       apply value_reduction_refl in H; simp_hyps; simplify_eq
   end.
 
-Lemma reduction_tlete:  forall e_x e α β (v : value),
-    α ⊧ tlete e_x e ↪*{ β } v ->
-    (exists (βx: trace) (v_x: value),
-      α ⊧ e_x ↪*{ βx } v_x /\ βx ⊧ (e ^t^ v_x) ↪*{ β } v).
+Lemma reduction_tlete:  forall e_x e (v : value),
+    tlete e_x e ↪* v -> (exists (v_x: value), e_x ↪* v_x /\ (e ^t^ v_x) ↪* v).
 Proof.
   intros.
   remember (tlete e_x e). remember (treturn v).
@@ -156,14 +150,14 @@ Proof.
   - repeat esplit. econstructor; eauto. eauto.
 Qed.
 
-Lemma reduction_tlete':  forall e_x e α βx βe (v_x v : value),
+Lemma reduction_tlete':  forall e_x e (v_x v : value),
     (* NOTE: This condition is unnecessary as it should be implied by the
     regularity lemma. Remove later when we bother proving a few more naming
     lemmas. *)
     body e ->
-    α ⊧ e_x ↪*{ βx } v_x ->
-    βx ⊧ (e ^t^ v_x) ↪*{ βe } v ->
-    α ⊧ tlete e_x e ↪*{ βe } v.
+    e_x ↪* v_x ->
+    (e ^t^ v_x) ↪* v ->
+    tlete e_x e ↪* v.
 Proof.
   intros * Hb H. remember (treturn v_x).
   induction H; intros; subst.
@@ -175,80 +169,123 @@ Proof.
     eauto.
 Qed.
 
-Lemma reduction_mk_app_e_v α β (f v_x v : value) :
+Lemma reduction_tlete_iff:
+  ∀ (e_x e : tm) (v : value),
+    tlete e_x e ↪* v
+    <-> (body e /\ ∃ (v_x : value),
+          e_x ↪* v_x ∧ e ^t^ v_x ↪* v).
+Proof.
+  split.
+  - split. apply multi_step_regular in H. simp_hyps. lc_solver.
+    apply reduction_tlete; eauto.
+  - intros. simp_hyps. eapply reduction_tlete'; eauto.
+Qed.
+
+Lemma reduction_mk_app_v_v (f v_x v : value) :
   lc v_x ->
-  α ⊧ mk_app_e_v f v_x ↪*{ β} v ->
-  α ⊧ tletapp f v_x (vbvar 0) ↪*{ β} v.
+  mk_app f v_x ↪* v ->
+  tletapp f v_x (vbvar 0) ↪* v.
 Proof.
   intros Hlc H.
   sinvert H. sinvert H0. easy.
+  sinvert H1. sinvert H. easy.
   simpl in *. simplify_list_eq.
-  rewrite open_rec_lc_value in * by eauto. eauto.
+  repeat rewrite open_rec_lc_value in * by eauto.
+  eauto.
 Qed.
 
-Lemma reduction_mk_app_e_v' α β (f v_x v : value) :
-  α ⊧ tletapp f v_x (vbvar 0) ↪*{ β} v ->
-  α ⊧ mk_app_e_v f v_x ↪*{ β} v.
+Lemma body_mk_app_aux2 (f: value): lc f -> body (tletapp f (vbvar 0) (vbvar 0)).
+Proof.
+  eexists. instantiate_atom_listctx.
+  simpl. apply letapp_lc_body. repeat split; eauto using lc.
+  by rewrite open_rec_lc_value.
+Qed.
+
+Lemma body_mk_app_aux v_x:
+  lc v_x ->
+  body (tlete v_x (tletapp (vbvar 1) (vbvar 0) (vbvar 0))).
+Proof.
+  eexists. instantiate_atom_listctx.
+  simpl. apply lete_lc_body. repeat split; eauto using lc.
+  by rewrite open_rec_lc_tm.
+Qed.
+
+Lemma reduction_mk_app_v_v' (f v_x v : value) :
+  tletapp f v_x (vbvar 0) ↪* v ->
+  mk_app f v_x ↪* v.
 Proof.
   intros H.
   assert (lc v_x). {
     apply multi_step_regular1 in H. sinvert H. eauto.
   }
+  assert (lc f). {
+    apply multi_step_regular1 in H. sinvert H. eauto.
+  }
   eapply_eq multistep_step.
   eapply STLetE2.
-  apply multi_step_regular1 in H. sinvert H. eauto.
+  - apply multi_step_regular1 in H. sinvert H. eauto.
   (* Probably should be a lemma. *)
-  eexists. instantiate_atom_listctx.
-  simpl. apply letapp_lc_body. repeat split; eauto using lc.
-  by rewrite open_rec_lc_value.
-  simpl. simplify_list_eq. rewrite open_rec_lc_value; eauto.
+  - apply body_mk_app_aux; eauto.
+  - simpl. simplify_list_eq. rewrite open_rec_lc_value; eauto.
+    eapply_eq multistep_step.
+    eapply STLetE2; eauto.
+    simpl. by rewrite open_rec_lc_value.
 Qed.
 
-Lemma reduction_letapplam α Tb e (v_x : value) β (v : value) :
+Lemma open_vlam_rev k Tb e (v: value): vlam Tb ({S k ~t> v} e) = {k ~v> v} vlam Tb e.
+Proof. eauto. Qed.
+
+Lemma reduction_mk_app_lam Tb e (v_x : value) (v : value) :
   lc v_x ->
-  α ⊧ mk_app_e_v (vlam Tb e) v_x ↪*{ β} v ->
-  α ⊧ e ^t^ v_x ↪*{ β} v.
+  mk_app (vlam Tb e) v_x ↪* v ->
+  e ^t^ v_x ↪* v.
 Proof.
-  intros Hlc H.
-  sinvert H.
-  sinvert H0; try easy.
-  simpl in H1.
-  rewrite open_rec_lc_value in H1 by auto.
+  unfold mk_app. intros Hlc H.
+  assert (lc (vlam Tb e)) as Haux. {
+    step_regular_simp. sinvert H; eauto.
+  }
+  apply reduction_tlete in H. simp_hyps. simpl in *.
+  rewrite open_rec_lc_value in H1; eauto.
+  apply value_reduction_refl in H0; sinvert H0.
+  apply reduction_tlete in H1. simp_hyps. simpl in *.
+  rewrite open_vlam_rev in H1.
+  rewrite open_rec_lc_value in H1; eauto.
+  apply value_reduction_refl in H0; sinvert H0.
   sinvert H1. sinvert H.
   apply reduction_tlete in H0.
   simp_hyps. simpl in *.
   eapply multistep_trans; eauto.
 Qed.
 
-Lemma reduction_letapplam' α Tb e (v_x : value) β (v : value) :
+Lemma reduction_mk_app_lam' Tb e (v_x : value) (v : value) :
   lc v_x ->
   (* NOTE: This condition is unnecessary as it should be implied by the
   regularity lemma. *)
   body e ->
-  α ⊧ e ^t^ v_x ↪*{ β} v ->
-  α ⊧ mk_app_e_v (vlam Tb e) v_x ↪*{ β} v.
+  e ^t^ v_x ↪* v ->
+  mk_app (vlam Tb e) v_x ↪* v.
 Proof.
-  intros Hlc Hb H.
-  eapply_eq multistep_step.
-  eapply STLetE2.
-  qauto using lc_abs_iff_body.
-  (* probably should be a lemma. *)
-  eexists. instantiate_atom_listctx.
-  simpl. apply letapp_lc_body. repeat split; eauto using lc.
-  by rewrite open_rec_lc_value.
-  simpl. econstructor.
-  econstructor. eauto. eauto.
-  by rewrite open_rec_lc_value.
-  rewrite open_rec_lc_value by eauto.
-  simplify_list_eq. eapply reduction_tlete'; eauto.
+  unfold mk_app. intros Hlc Hb H.
+  assert (lc (vlam Tb e)) as Haux by lc_solver.
+  apply reduction_tlete' with (v_x := vlam Tb e); eauto.
+  apply body_mk_app_aux; eauto.
+  simpl. rewrite open_rec_lc_value; eauto.
+  apply reduction_tlete' with (v_x := v_x); eauto.
+  simpl. rewrite open_vlam_rev; rewrite open_rec_lc_value; eauto.
+  eapply_eq multistep_step. econstructor; eauto.
+  apply reduction_tlete' with (v_x := v); eauto.
   simpl. econstructor. eauto using multi_step_regular2.
 Qed.
 
-Lemma reduction_tletapp:  forall v1 v2 e α β (v : value),
-    α ⊧ tletapp v1 v2 e ↪*{ β} v ->
-    (exists (βx: trace) (v_x: value),
-      α ⊧ mk_app_e_v v1 v2 ↪*{ βx } v_x /\
-        βx ⊧ (e ^t^ v_x) ↪*{ β } v).
+Ltac value_reduction_simp :=
+  repeat
+    match goal with
+    | [H: treturn _ ↪* treturn _ |- _ ] => apply value_reduction_refl in H; sinvert H
+    end.
+
+Lemma reduction_tletapp:  forall v1 v2 e (v : value),
+    tletapp v1 v2 e ↪* v ->
+    (exists (v_x: value), tletapp v1 v2 (vbvar 0) ↪* v_x /\ (e ^t^ v_x) ↪* v).
 Proof.
   intros.
   remember (tletapp v1 v2 e). remember (treturn v).
@@ -258,52 +295,86 @@ Proof.
   simp_hyps. sinvert H.
   - eapply reduction_tlete in H0. simp_hyps.
     simplify_list_eq.
-    eexists _, _. repeat split; eauto using reduction_letapplam'.
+    eexists _. repeat split; eauto using reduction_mk_app_lam'.
+    eapply_eq multistep_step. econstructor; eauto.
+    eapply reduction_tlete'; eauto. simpl.
+    econstructor. apply multi_step_regular2 in H0; eauto.
   - simplify_list_eq.
     ospecialize* H1; eauto. simp_hyps.
-    eexists _, _.
+    eexists _.
     repeat split; cycle 1; eauto.
-
-    (* Maybe this should be a lemma about [vfix]. *)
-    apply reduction_mk_app_e_v in H.
-    apply reduction_mk_app_e_v'.
-    econstructor. econstructor; eauto.
-    simplify_list_eq. eauto.
-    apply multi_step_regular1 in H0.
-    sinvert H0. eauto.
+    eapply_eq multistep_step. econstructor; eauto.
+    simpl. eauto.
 Qed.
 
-Lemma value_reduction_refl': forall (v1: value) v2, (∀ α, α ⊧ v1 ↪*{ α} v2) -> v2 = v1.
+Lemma reduction_tletapp':  forall v1 v2 e (v : value),
+    (body e /\ exists (v_x: value), tletapp v1 v2 (vbvar 0) ↪* v_x /\ (e ^t^ v_x) ↪* v) -> tletapp v1 v2 e ↪* v.
 Proof.
-  intros * H. specialize (H []).
-  sinvert H; easy.
+  intros. destruct H as (He & (v_x & Hv_x & H)).
+  remember (tletapp v1 v2 (vbvar 0)). remember (treturn v_x).
+  generalize dependent v2.
+  generalize dependent v1.
+  generalize dependent v_x.
+  induction Hv_x; intros; subst. easy.
+  simp_hyps. sinvert H.
+  - clear IHHv_x.
+    eapply reduction_tlete in Hv_x. simp_hyps.
+    simplify_list_eq. value_reduction_simp.
+    eapply_eq multistep_step. econstructor; eauto.
+    eapply reduction_tlete'; eauto.
+  - simplify_list_eq.
+    ospecialize* IHHv_x; eauto.
+    eapply_eq multistep_step. econstructor; eauto.
+    simpl. eauto.
 Qed.
 
-Lemma value_reduction_any_ctx: forall (v1: value) α, lc v1 -> α ⊧ v1 ↪*{ α} v1.
+Lemma reduction_tletapp_iff:  forall v1 v2 e (v : value),
+    tletapp v1 v2 e ↪* v <-> (body e /\ exists (v_x: value), tletapp v1 v2 (vbvar 0) ↪* v_x /\ (e ^t^ v_x) ↪* v).
+Proof.
+  split; intros.
+  - split. apply multi_step_regular1 in H. lc_solver.
+    apply reduction_tletapp; eauto.
+  - apply reduction_tletapp'; eauto.
+Qed.
+
+Lemma value_reduction_any_ctx: forall (v1: value), lc v1 -> v1 ↪* v1.
 Proof.
   intros. econstructor; eauto.
 Qed.
 
-Lemma reduction_tleteffop:  forall op v2 e α β (v : value),
-    α ⊧ (tleteffop op v2 e) ↪*{ β} v ->
-    exists (c2 c_x: constant) βx,
-      v2 = c2 /\ α ⊧{op ~ c2}⇓{ βx }{ c_x } /\ βx ⊧ (e ^t^ c_x) ↪*{ β} v.
+Lemma reduction_tleteffop:  forall op v2 e (v : value),
+    (tleteffop op v2 e) ↪* v ->
+    exists (c2 c_x: constant),
+      v2 = c2 /\ ⇓{op ~ c2}{ c_x } /\ (e ^t^ c_x) ↪* v.
 Proof.
   intros.
   sinvert H. sinvert H0.
   eauto 10.
 Qed.
 
-Lemma reduction_matchb_true:  forall e1 e2 α β (v : value),
-    α ⊧ tmatchb true e1 e2 ↪*{ β} v -> α ⊧ e1 ↪*{ β} v.
+
+Lemma reduction_tleteffop_iff:  forall op v2 e (v : value),
+    (tleteffop op v2 e) ↪* v <->
+      body e /\ exists (c2 c_x: constant),
+        v2 = c2 /\ ⇓{op ~ c2}{ c_x } /\ (e ^t^ c_x) ↪* v.
+Proof.
+  split.
+  - intuition.
+    + apply multi_step_regular in H. simp_hyps. rewrite leteffop_lc_body in H. intuition.
+    + apply reduction_tleteffop; eauto.
+  - intros. simp_hyps. subst. repeat (econstructor; eauto).
+Qed.
+
+Lemma reduction_matchb_true:  forall e1 e2 (v : value),
+    tmatchb true e1 e2 ↪* v -> e1 ↪* v.
 Proof.
   intros.
   sinvert H.
   sinvert H0. simplify_list_eq. eauto.
 Qed.
 
-Lemma reduction_matchb_false:  forall e1 e2 α β (v : value),
-    α ⊧ tmatchb false e1 e2 ↪*{ β} v -> α ⊧ e2 ↪*{ β} v.
+Lemma reduction_matchb_false:  forall e1 e2 (v : value),
+    tmatchb false e1 e2 ↪* v -> e2 ↪* v.
 Proof.
   intros.
   sinvert H.
@@ -314,8 +385,8 @@ Qed.
 
 Ltac lc_solver_simp_aux :=
   match goal with
-  | [H: _ ⊧ _ ↪*{ _ } _ |- lc _] => apply multi_step_regular in H; simp_hyps
-  | [H: _ ⊧ _ ↪*{ _ } _ |- body _] => apply multi_step_regular in H; simp_hyps
+  | [H: _ ↪* _ |- lc _] => apply multi_step_regular in H; simp_hyps
+  | [H: _ ↪* _ |- body _] => apply multi_step_regular in H; simp_hyps
   end.
 
 Ltac lc_solver_simp :=
@@ -328,22 +399,22 @@ Ltac lc_solver_plus_aux :=
   end.
 
 Ltac lc_solver_plus :=
-  lc_solver_simp; eauto;
+  eauto; lc_solver_simp; eauto;
   (repeat lc_solver_plus_aux); eauto.
 
 Lemma reduction_tlete_value: forall (v1: value) e2,
-  forall α β (v: value), α ⊧ tlete v1 e2 ↪*{ β} v <-> (lc v1 /\ body e2 /\ α ⊧ e2 ^t^ v1 ↪*{ β} v).
+  forall (v: value), tlete v1 e2 ↪* v <-> (lc v1 /\ body e2 /\ e2 ^t^ v1 ↪* v).
 Proof.
   split; intros.
   - assert (lc v1) by lc_solver_plus.
-    assert (body e2) by lc_solver_plus.
+    assert (body e2) by lc_solver_plus. intuition.
     apply reduction_tlete in H. simp_hyps.
-    apply value_reduction_refl in H. simp_hyps. subst; intuition.
+    apply value_reduction_refl in H2. simp_hyps. subst; intuition.
   - simp_hyps. eapply reduction_tlete'; eauto.
 Qed.
 
 Lemma reduction_nest_tlete: forall e,
-  forall α β (v: value), α ⊧ tlete e (vbvar 0) ↪*{ β} v <-> α ⊧ e ↪*{ β} v.
+  forall (v: value), tlete e (vbvar 0) ↪* v <-> e ↪* v.
 Proof.
   intros e. split; intros.
   - apply reduction_tlete in H. simp_hyps. simpl in *.
@@ -354,9 +425,9 @@ Proof.
     apply multi_step_regular2 in H; eauto.
 Qed.
 
-Lemma reduction_tletapp_lam:  forall T e1 v2 e α β (v : value),
-    α ⊧ tletapp (vlam T e1) v2 e ↪*{ β} v <->
-      (lc v2 /\ lc (vlam T e1) /\ α ⊧ tlete (e1 ^t^ v2) e ↪*{ β} v).
+Lemma reduction_tletapp_lam:  forall T e1 v2 e (v : value),
+    tletapp (vlam T e1) v2 e ↪* v <->
+      (lc v2 /\ lc (vlam T e1) /\ tlete (e1 ^t^ v2) e ↪* v).
 Proof.
   split; intros.
   - inversion H; subst. inversion H0; subst; eauto.
@@ -367,9 +438,9 @@ Proof.
     econstructor; eauto. lc_solver.
 Qed.
 
-Lemma reduction_tletapp_fix:  forall T_f (v_x: value) (e1: tm) e (v : value) α β,
-      α ⊧ tletapp (vfix T_f (vlam T_f e1)) v_x e ↪*{ β} v <->
-        (lc v_x /\ α ⊧ tletapp ((vlam T_f e1) ^v^ v_x) (vfix T_f (vlam T_f e1)) e ↪*{ β} v).
+Lemma reduction_tletapp_fix:  forall T_f (v_x: value) (e1: tm) e (v : value),
+      tletapp (vfix T_f (vlam T_f e1)) v_x e ↪* v <->
+        (lc v_x /\ tletapp ((vlam T_f e1) ^v^ v_x) (vfix T_f (vlam T_f e1)) e ↪* v).
 Proof.
   split; intros.
   - inversion H; subst. inversion H0; subst; eauto.
@@ -380,79 +451,23 @@ Proof.
     lc_solver. lc_solver.
 Qed.
 
-Lemma reduction_mk_app_e_v_f:  forall e α β (v_x v : value),
-    lc v_x ->
-    α ⊧ mk_app_e_v e v_x ↪*{ β} v <->
-      (exists (f: value) γ, α ⊧ e ↪*{ γ} f /\ γ ⊧ mk_app_e_v f v_x ↪*{ β} v).
+Lemma reduction_mk_app_iff:  forall e e_x (v : value),
+    lc e_x ->
+    mk_app e e_x ↪* v <->
+      (exists (f v_x: value), e ↪* f /\ e_x ↪* v_x /\ tletapp f v_x (vbvar 0) ↪* v).
 Proof.
-  intros e α β v_x v Hlc.
-  unfold mk_app_e_v.
+  intros e e_x v Hlc.
+  unfold mk_app.
   split; intros.
-  - assert (body (tletapp (vbvar 0) v_x (vbvar 0))) by lc_solver_plus.
-    apply reduction_tlete in H. destruct H as (γ & f & Hf & Hv).
-    exists f. exists γ. intuition. simpl in Hv.
-    assert (γ ⊧ f ↪*{ γ} f). {
-      apply value_reduction_any_ctx. lc_solver_plus.
-    }
-    eapply reduction_tlete'; eauto.
-  - simp_hyps.
-    eapply reduction_tlete'; eauto. lc_solver_plus.
-    rewrite reduction_tlete_value in H1. simp_hyps. eauto.
-Qed.
-
-Lemma reduction_tlete_iff:
-  ∀ (e_x e : tm) (α β : list evop) (v : value),
-    α ⊧ tlete e_x e ↪*{ β} v
-    <-> (body e /\ ∃ (βx : trace) (v_x : value),
-          α ⊧ e_x ↪*{ βx} v_x ∧ βx ⊧ e ^t^ v_x ↪*{ β} v).
-Proof.
-  split.
-  - split. apply multi_step_regular in H. simp_hyps. lc_solver.
-    apply reduction_tlete; eauto.
-  - intros. simp_hyps. eapply reduction_tlete'; eauto.
-Qed.
-
-Lemma reduction_tletapp': forall (v1 v2: value) e α β (v : value),
-    (body e /\ lc v2 /\ exists (βx: trace) (v_x: value),
-        α ⊧ mk_app_e_v v1 v2 ↪*{ βx } v_x /\
-          βx ⊧ (e ^t^ v_x) ↪*{ β } v) ->
-    α ⊧ tletapp v1 v2 e ↪*{ β} v.
-Proof.
-  intros. destruct H as (Hlc1 & Hlc2 & βx & v_x & Hst1 & Hst2).
-  apply reduction_mk_app_e_v in Hst1; eauto.
-  sinvert Hst1. sinvert H.
-  - rewrite reduction_nest_tlete in H0.
-    rewrite reduction_tletapp_lam. intuition. lc_solver.
-    erewrite reduction_tlete_iff. intuition; eauto.
-  - rewrite reduction_tletapp_fix. intuition.
-    simpl in *. rewrite reduction_tletapp_lam in H0.
-    rewrite reduction_tletapp_lam. intuition.
-    rewrite reduction_nest_tlete in H2.
-    erewrite reduction_tlete_iff. intuition; eauto.
-Qed.
-
-Lemma reduction_tletapp_iff: forall (v1 v2: value) e α β (v : value),
-    α ⊧ tletapp v1 v2 e ↪*{ β} v <->
-    (body e /\ lc v2 /\ exists (βx: trace) (v_x: value),
-        α ⊧ mk_app_e_v v1 v2 ↪*{ βx } v_x /\
-          βx ⊧ (e ^t^ v_x) ↪*{ β } v).
-Proof.
-  split.
-  - intros. intuition.
-    + apply multi_step_regular in H. simp_hyps. lc_solver.
-    + apply multi_step_regular in H. simp_hyps. lc_solver.
-    + apply reduction_tletapp; eauto.
-  - apply reduction_tletapp'.
-Qed.
-
-Lemma reduction_tleteffop_iff:  forall op v2 e α β (v : value),
-    α ⊧ (tleteffop op v2 e) ↪*{ β} v <->
-    body e /\ exists (c2 c_x: constant) βx,
-      v2 = c2 /\ α ⊧{op ~ c2}⇓{ βx }{ c_x } /\ βx ⊧ (e ^t^ c_x) ↪*{ β} v.
-Proof.
-  split.
-  - intuition.
-    + apply multi_step_regular in H. simp_hyps. rewrite leteffop_lc_body in H. intuition.
-    + apply reduction_tleteffop; eauto.
-  - intros. simp_hyps. subst. repeat (econstructor; eauto).
+  - apply reduction_tlete in H. destruct H as (f & Hf & H).
+    simpl in H. rewrite open_rec_lc_tm in H by eauto.
+    apply reduction_tlete in H. destruct H as (v_x & Hv_x & H).
+    simpl in H. rewrite open_rec_lc_value in H by lc_solver_plus.
+    exists f, v_x. intuition.
+  - destruct H as (f & v_x & Hf & Hv_x & H).
+    eapply reduction_tlete'; eauto. apply body_mk_app_aux; eauto.
+    simpl. rewrite open_rec_lc_tm; eauto.
+    eapply reduction_tlete'; eauto. apply body_mk_app_aux2. by lc_solver_plus.
+    simpl. rewrite open_rec_lc_value; eauto.
+    all: by lc_solver_plus.
 Qed.
