formalization/Instantiation.v
@@ -4,7 +4,6 @@ From CT Require Import CoreLangProp.
 From CT Require Import OperationalSemantics.
 From CT Require Import BasicTypingProp.
 From CT Require Import Qualifier.
-From CT Require Import Transducer.
 From CT Require Import RefinementType.
 
 Import Atom.
@@ -13,8 +12,6 @@ Import Tactics.
 Import NamelessTactics.
 Import OperationalSemantics.
 Import BasicTyping.
-Import Trace.
-Import Transducer.
 Import RefinementType.
 
 (** This file defines valuation environment, i.e., substitution (σ), and
@@ -22,6 +19,7 @@ Import RefinementType.
 
 (** Environment (substitution) *)
 Notation env := (amap value).
+Notation pp := ((amap value) -> Prop).
 
 Definition closed_env (env : env) := map_Forall (fun _ => closed_value) env.
 
@@ -32,7 +30,6 @@ Definition msubst {A} (subst : atom -> value -> A -> A)
   map_fold subst a env.
 
 Notation "'m{' x '}q'" := (msubst qualifier_subst x) (at level 20, format "m{ x }q", x constr).
-Notation "'m{' x '}a'" := (msubst td_subst x) (at level 20, format "m{ x }a", x constr).
 Notation "'m{' x '}r'" := (msubst rty_subst x) (at level 20, format "m{ x }r", x constr).
 Notation "'m{' x '}v'" := (msubst value_subst x) (at level 20, format "m{ x }v", x constr).
 Notation "'m{' x '}t'" := (msubst tm_subst x) (at level 20, format "m{ x }t", x constr).
